example_chat.thy
@@ -609,6 +609,7 @@ proof M_show_programCorrect
             if tx_fresh: "\<And>tx. s_transactionOrigin tx \<noteq> Some i"
               and inv_initial: "invariant progr \<lparr>calls = s_calls, happensBefore = s_happensBefore, callOrigin = s_callOrigin, transactionOrigin = s_transactionOrigin, knownIds = s_knownIds, invocationOp = s_invocationOp(i \<mapsto> SendMessage author content), invocationRes = s_invocationRes(i := None)\<rparr>"
             for  s_calls s_happensBefore s_callOrigin s_transactionOrigin s_knownIds s_invocationOp s_invocationRes
+            apply repliss_vcg_l
           proof (repliss_vcg_l, goal_cases "AtCommit" "AtReturn" )
             case (AtCommit v tx s_calls' s_happensBefore' s_callOrigin' s_transactionOrigin' s_knownIds' vis' s_invocationOp' s_invocationRes' c res ca resa cb resb)
 
